Examples/Kruskal/Kruskal.thy
@@ -30,9 +30,9 @@ locale Kruskal_intermediate = Kruskal_intermediate_defs   E forest connected pat
    and connected :: "('a uprod) set \<Rightarrow> ('a*'a) set"
    and path :: "('a uprod) set \<Rightarrow> 'a \<Rightarrow> ('a uprod) list \<Rightarrow> 'a \<Rightarrow> bool"
    and weight :: "'a uprod \<Rightarrow> 'b::{linorder, ordered_comm_monoid_add}" +
- fixes   sorted_carrier_time :: nat
-    and  empty_forest_time indep_test_time insert_time :: nat 
-    and getEdges_time :: nat
+ fixes     
+       empty_forest_time indep_test_time insert_time :: nat 
+    and getEdges_time sort_time :: nat 
  assumes Eproper: "\<And>e. e\<in>E \<Longrightarrow> proper_uprod e" 
    and finiteE[simp]: "finite E" 
    and forest_subE: "forest E' \<Longrightarrow> E' \<subseteq> E"
@@ -188,7 +188,7 @@ proof -
     by blast
 qed
 
-sublocale minWeightBasis E forest weight       sorted_carrier_time
+sublocale minWeightBasis E forest weight       "getEdges_time + sort_time"
      empty_forest_time indep_test_time insert_time 
 proof  
   have "forest {}" using forest_empty by auto
