Examples/Kruskal/Kruskal_Impl.thy
@@ -1,0 +1,199 @@
+theory Kruskal_Impl
+imports Kruskal_Refine "../../Refine_Imperative_HOL/Sepref"
+begin
+
+
+
+definition "sort_edges \<equiv> quicksort_by_rel edges_less_eq []"
+
+
+definition "max_node l \<equiv> Max (insert 0 (fst`set l \<union> (snd o snd)`set l))"
+
+lemma max_node_impl[code]: "max_node l = fold (\<lambda>(u,_,w) x. max u (max w x)) l 0"
+proof -
+  have "fold (\<lambda>(u,_,w) x. max u (max w x)) l a = Max (insert a (fst`set l \<union> (snd o snd)`set l))" for a
+    apply (induction l arbitrary: a)
+    apply (auto simp:  )
+    subgoal for a b l aa
+      apply (cases l)
+      by (auto simp: ac_simps)
+    done
+  thus ?thesis unfolding max_node_def by auto
+qed
+
+lemma set_uprod_nonempty[simp]: "set_uprod x \<noteq> {}"
+  apply(cases x) by auto
+
+locale Kruskal_intermediate_Impl = Kruskal_intermediate E forest connected path weight for E forest connected path 
+      and weight :: "nat uprod \<Rightarrow> int"  +
+    fixes getEdges  :: "(nat \<times> int \<times> nat) list nres"
+      and getEdges_impl :: "(nat \<times> int \<times> nat) list Heap"
+    assumes  
+        getEdges_refine: "getEdges \<le> SPEC (\<lambda>L. lst_graph_P' weight L E)"
+      and
+        getEdges_impl: "(uncurry0 getEdges_impl, uncurry0 getEdges) \<in> unit_assn\<^sup>k \<rightarrow>\<^sub>a list_assn (nat_assn \<times>\<^sub>a int_assn \<times>\<^sub>a nat_assn)"
+      and
+         E_nonempty: "E\<noteq>{}"
+begin
+
+
+
+
+       
+definition "obtain_sorted_carrier''' =
+      do {
+    l \<leftarrow> getEdges;
+    RETURN (quicksort_by_rel edges_less_eq [] l, max_node l)
+}" 
+
+definition "is_linorder_rel R \<equiv> (\<forall>x y. R x y \<or> R y x) \<and> (\<forall>x y z. R x y \<longrightarrow> R y z \<longrightarrow> R x z)"
+lemma edges_less_eq_linorder: "is_linorder_rel edges_less_eq"
+  unfolding edges_less_eq_def is_linorder_rel_def
+  by (metis linear order_trans)
+lemma sort_edges_correct: "sorted_wrt edges_less_eq (quicksort_by_rel edges_less_eq [] l)"
+  by (metis (no_types, hide_lams) edges_less_eq_linorder is_linorder_rel_def sorted_wrt_quicksort_by_rel)
+
+lemma distinct_mset_eq:"distinct a \<Longrightarrow> mset a = mset b \<Longrightarrow> distinct b"
+  by (metis card_distinct distinct_card set_mset_mset size_mset)
+
+lemma quicksort_by_rel_distinct: "distinct l \<Longrightarrow> distinct (quicksort_by_rel edges_less_eq [] l)"
+  by (auto intro: distinct_mset_eq)
+
+definition "add_size_rel   = br fst (\<lambda>(l,n). n= Max V)"
+
+
+
+lemma max_node_is_Max_V: " E = (\<lambda>(a, _, y). Upair a y) ` set la \<Longrightarrow> max_node la = Max V"
+proof -
+  assume E: "E = (\<lambda>(a, _, y). Upair a y) ` set la"
+  have pff: "fst ` set la \<union> (snd \<circ> snd) ` set la = (\<Union>x\<in>set la. case x of (x1, x1a, x2a) \<Rightarrow> {x1, x2a})"
+    apply auto by (metis image_comp img_snd)
+  have "V \<noteq> {}" using E_nonempty V_def by auto
+  then have Mo: "Max V = Max (insert 0 V)" by auto
+  show ?thesis unfolding Mo unfolding V_def
+  unfolding E apply simp 
+  by (auto simp add:  max_node_def prod.case_distrib pff ) 
+qed
+
+
+lemma obtain_sorted_carrier'''_refine: "(obtain_sorted_carrier''', obtain_sorted_carrier'') \<in> \<langle>add_size_rel\<rangle>nres_rel"
+  unfolding obtain_sorted_carrier'''_def obtain_sorted_carrier''_def
+  apply(refine_rcg getEdges_refine)  
+  by (auto intro!: RETURN_SPEC_refine simp:   quicksort_by_rel_distinct sort_edges_correct
+          add_size_rel_def in_br_conv lst_graph_P_def max_node_is_Max_V
+         dest!: distinct_mapI)
+
+ definition kruskal3 :: "(nat \<times> int \<times> nat) list nres"
+   where "kruskal3  \<equiv> do {
+    (sl,mn) \<leftarrow> obtain_sorted_carrier''';
+    let initial_union_find = per_init' (mn + 1);
+    (per, spanning_forest) \<leftarrow> nfoldli sl (\<lambda>_. True)
+        (\<lambda>(a,w,b) (uf, T). do { 
+            ASSERT (a \<in> Domain uf \<and> b \<in> Domain uf);
+            if \<not> per_compare uf a b then
+              do { 
+                let uf = per_union uf a b;
+                ASSERT ((a,w,b)\<notin>set T);
+                RETURN (uf, T@[(a,w,b)])
+              }
+            else 
+              RETURN (uf,T)
+        }) (initial_union_find, []);
+        RETURN spanning_forest
+      }"
+
+
+  definition per_supset_rel :: "('a per \<times> 'a per) set" where
+    "per_supset_rel
+      \<equiv> {(p1,p2). p1 \<inter> Domain p2 \<times> Domain p2 = p2 \<and> p1 - (Domain p2 \<times> Domain p2) \<subseteq> Id}"
+
+  lemma per_supset_rel_dom: "(p1, p2) \<in> per_supset_rel \<Longrightarrow> Domain p1 \<supseteq> Domain p2"
+    by (auto simp: per_supset_rel_def)
+  
+  lemma per_supset_compare:
+    "(p1, p2) \<in> per_supset_rel \<Longrightarrow> x1\<in>Domain p2 \<Longrightarrow> x2\<in>Domain p2 \<Longrightarrow> per_compare p1 x1 x2 \<longleftrightarrow> per_compare p2 x1 x2"
+    by (auto simp: per_supset_rel_def)
+  
+  lemma per_supset_union: "(p1, p2) \<in> per_supset_rel \<Longrightarrow> x1\<in>Domain p2 \<Longrightarrow> x2\<in>Domain p2 \<Longrightarrow>
+    (per_union p1 x1 x2, per_union p2 x1 x2) \<in> per_supset_rel"
+    apply (clarsimp simp: per_supset_rel_def per_union_def Domain_unfold )
+    apply (intro subsetI conjI)
+    apply blast
+    apply force
+    done
+
+lemma per_initN_refine: "(per_init' (Max V + 1), per_init V) \<in> per_supset_rel"
+  unfolding per_supset_rel_def per_init'_def per_init_def max_node_def
+  by (auto simp: less_Suc_eq_le  ) 
+
+theorem kruskal3_refine: "(kruskal3, kruskal2)\<in>\<langle>Id\<rangle>nres_rel"
+  unfolding kruskal2_def kruskal3_def Let_def
+  apply (refine_rcg obtain_sorted_carrier'''_refine[THEN nres_relD]   )
+  supply RELATESI[where R="per_supset_rel::(nat per \<times> _) set", refine_dref_RELATES]
+         apply refine_dref_type 
+         apply (simp add: add_size_rel_def in_br_conv)
+  using per_initN_refine apply (simp add: add_size_rel_def in_br_conv)
+  by (auto simp add: add_size_rel_def in_br_conv per_supset_compare
+                per_supset_union
+             dest: per_supset_rel_dom
+             simp del: per_compare_def )
+ 
+
+
+
+section \<open>Kruskal\<close>
+
+
+lemma [sepref_import_param]: "(sort_edges,sort_edges)\<in>\<langle>Id\<times>\<^sub>rId\<times>\<^sub>rId\<rangle>list_rel \<rightarrow>\<langle>Id\<times>\<^sub>rId\<times>\<^sub>rId\<rangle>list_rel" by simp
+lemma [sepref_import_param]: "(max_node, max_node) \<in> \<langle>Id\<times>\<^sub>rId\<times>\<^sub>rId\<rangle>list_rel \<rightarrow> nat_rel" by simp
+
+  sepref_register "getEdges" :: "(nat \<times> int \<times> nat) list nres"
+ 
+ 
+declare getEdges_impl [sepref_fr_rules]
+
+sepref_definition kruskal is
+  "uncurry0 kruskal3" :: "(unit_assn)\<^sup>k \<rightarrow>\<^sub>a list_assn (nat_assn \<times>\<^sub>a int_assn \<times>\<^sub>a nat_assn)"
+  unfolding kruskal3_def obtain_sorted_carrier'''_def 
+  unfolding sort_edges_def[symmetric]
+  apply (rewrite at "nfoldli _ _ _ (_,\<hole>)" HOL_list.fold_custom_empty)
+  by sepref 
+
+thm kruskal3_refine kruskal2_refine   kruskal1_refine kruskal0_refine minWeightBasis3_refine
+
+abbreviation "MST == minBasis"
+
+(* TODO: *) 
+
+lemmas kruskal3_ref_spec = kruskal3_refine[FCOMP kruskal2_refine,
+            FCOMP kruskal1_refine,
+            FCOMP kruskal0_refine,
+            FCOMP minWeightBasis3_refine] 
+
+  lemma [fcomp_norm_simps]: "list_assn (nat_assn \<times>\<^sub>a int_assn \<times>\<^sub>a nat_assn) = id_assn"
+    by (auto simp: list_assn_pure_conv)
+lemmas kruskal_ref_spec = kruskal.refine[FCOMP kruskal3_ref_spec]
+
+
+lemma kruskal_correct_forest:
+  shows "<emp> kruskal <\<lambda>r. \<up>( MST (set (map \<alpha>' r)))>\<^sub>t"
+proof -
+  show ?thesis
+    using kruskal_ref_spec[to_hnr]
+    unfolding hn_refine_def lst_graph_rel_alt
+    apply clarsimp
+    apply (erule cons_post_rule)
+    by (sep_auto simp: hn_ctxt_def pure_def list_set_rel_def in_br_conv
+              dest: list_relD)     
+qed
+
+ 
+
+
+
+
+end
+
+
+
+end
